

On the problem of PCE's

We have the matrix

$$M = \begin{pmatrix} 1 & 1 & 1 & 1 \\ 1 & 1 & -1 & -1 \\ 1 & -1 & 1 & -1 \\ 1 & -1 & -1 & 1 \end{pmatrix} \quad (1)$$

which satisfies the obvious relation

$$M^{-1} = \frac{1}{2}M \quad (2)$$

We wish to find those vectors consisting of 0's and 1's such that

$$M^{\otimes N} \vec{\sigma} \quad (3)$$

is a vector with positive entries. Here $\vec{\sigma}$ is a 4^N dimensional vector of 0's and 1's. We number the entries of $\vec{\sigma}$ by the multi-indices $\vec{\alpha} = (\alpha_1, \dots, \alpha_N)$ where $0 \leq \alpha_k \leq 4$. The entries of the positive vector are given by $2^N p_{\vec{\alpha}}$. It then follows that the expression (3) satisfies

$$\left(M_{\vec{\alpha}\vec{\beta}}^{\otimes N} \right) \sigma_{\beta} = 2^N p_{\alpha} \quad (4)$$

where clearly

$$\left(M_{\vec{\alpha}\vec{\beta}}^{\otimes N} \right) = M_{\alpha_1 \beta_1} \cdot \dots \cdot M_{\alpha_N \beta_N} \quad (5)$$

From (4) immediately follows, via (2)

$$\sigma_{\alpha} = \left(M_{\vec{\alpha}\vec{\beta}}^{\otimes N} \right) p_{\beta} \quad (6)$$

which we analyze iteratively. We shall essentially use the fact that

$$p_{\vec{\alpha}} + p_{\vec{\beta}} = 0 \quad \Leftrightarrow \quad p_{\vec{\alpha}} = p_{\vec{\beta}} = 0 \quad (7)$$

Now we need a definition: to each multi-index $\vec{\alpha}$ we associate a *set* of multi-indices $\Phi(\vec{\alpha})$ as follows

$$\Phi(\vec{\alpha}) := \left\{ \vec{\beta} : \left(M^{\otimes N} \right)_{\vec{\alpha}\vec{\beta}} = 1 \right\} = \left\{ \vec{\beta} : M_{\alpha_1 \beta_1} \cdot \dots \cdot M_{\alpha_N \beta_N} = 1 \right\} \quad (8)$$

If we now assume that $\sigma_{\vec{\alpha}} = 1$, it follows from subtracting the two combined equations

$$\sum_{\vec{\beta}} p_{\vec{\beta}} = 1 \quad (9a)$$

$$\sum_{\vec{\beta}} \left(M^{\otimes N} \right)_{\vec{\alpha}\vec{\beta}} p_{\vec{\beta}} = \sigma_{\vec{\alpha}} = 1 \quad (9b)$$

that for all $\vec{\beta} \notin \Phi(\vec{\alpha})$

$$p_{\vec{\beta}} = 0. \quad (10)$$

From this follows that $\sigma_{\vec{\alpha}} = 1$ implies various equalities between the remaining $\sigma_{\vec{\gamma}}$. Indeed, let

$$(M^{\otimes N})_{\vec{\beta}\vec{\gamma}} = (M^{\otimes N})_{\vec{\beta}\vec{\gamma}'} \quad (11)$$

hold for all $\vec{\beta} \in \Phi(\vec{\alpha})$. If this condition is fulfilled and $\sigma_{\vec{\alpha}} = 1$, then

$$\sigma_{\vec{\gamma}} = \sum_{\vec{\beta}} (M^{\otimes N})_{\vec{\beta}\vec{\gamma}} p_{\vec{\beta}} \quad (12a)$$

$$= \sum_{\vec{\beta} \in \Phi(\vec{\alpha})} (M^{\otimes N})_{\vec{\beta}\vec{\gamma}} p_{\vec{\beta}} \quad (12b)$$

$$= \sum_{\vec{\beta} \in \Phi(\vec{\alpha})} (M^{\otimes N})_{\vec{\beta}\vec{\gamma}'} p_{\vec{\beta}} \quad (12c)$$

$$= \sum_{\vec{\beta}} (M^{\otimes N})_{\vec{\beta}\vec{\gamma}'} p_{\vec{\beta}} \quad (12d)$$

$$= \sigma_{\vec{\gamma}'} \quad (12e)$$

Here the transition from (12a) to (12b) follows from (10), from (12b) to (12c) follows from (11), from (12c) to (12d) follows again from (10).

Condition (11) combined with $\sigma_{\vec{\alpha}} = 1$ therefore implies $\sigma_{\vec{\gamma}} = \sigma_{\vec{\gamma}'}$. Since $M_{\alpha\beta} = \pm 1$, we may rewrite (11) as

$$M_{\beta_1\gamma_1} M_{\beta_1\gamma'_1} \cdots M_{\beta_N\gamma_N} M_{\beta_N\gamma'_N} = 1. \quad (13)$$

This must hold for all $\vec{\beta} \in \Phi(\vec{\alpha})$. From this follows that (13) may be rewritten as

$$M_{\beta_1\gamma_1} M_{\beta_1\gamma'_1} \cdots M_{\beta_N\gamma_N} M_{\beta_N\gamma'_N} = M_{\alpha_1\beta_1} \cdots M_{\alpha_N\beta_N}. \quad (14)$$

Since this must hold for all $\vec{\beta} \in \Phi(\vec{\alpha})$, it follows that for all $1 \leq k \leq N$, γ_k and γ'_k are so related that

$$M_{\beta\gamma_k} M_{\beta\gamma'_k} = M_{\beta\alpha} \quad (15)$$

for all $0 \leq \beta \leq 3$. This is equivalently expressed as

$$M_{\beta\gamma'_k} = M_{\beta\gamma_k} M_{\beta\alpha} \quad (16)$$

which we further express as

$$\gamma'_k = \alpha \oplus \gamma_k \quad (17)$$

where the \oplus operation is defined by (16). See Figure 1 for a detailed description.

Now everything follows with delightful simplicity. First extend the \oplus operation to vectors componentwise

$$\vec{\alpha} \oplus \vec{\beta} = (\alpha_1 \oplus \beta_1, \dots, \alpha_N \oplus \beta_N). \quad (18)$$

\oplus	0	1	2	3
0	0	1	2	3
1	1	0	3	2
2	2	3	0	1
3	3	2	1	0

Figure 1: Table for the \oplus operation defined in (16). Note that the operation is an *abelian group*, in fact it corresponds to the *Klein group*, where the neutral element is 0. This is the reason for choosing an additive notation for the operation defined in (16).

Remark, as a useful fact, that the inverse under \oplus of any number α is α itself. If $\sigma_{\vec{\alpha}} = 1$, then it follows from the above that for all γ

$$\sigma_{\vec{\gamma}} = \sigma_{\vec{\alpha} \oplus \vec{\gamma}}. \quad (19)$$

So we may now proceed to generate all solutions: we start out from the solution having $\sigma_{\vec{0}} = 1$, with everything else 0. We may then successively switch σ 's to 1 for various values of $\vec{\alpha}$, taking care immediately to set equal to one the values of σ that correspond to values of $\vec{\beta}$ generated by the previously switched values of $\vec{\alpha}$ via (19).

We may now interpret this a bit differently: (19) states that the set of all $\vec{\alpha}$'s for which $\sigma_{\vec{\alpha}} = 1$ is closed under the operation \oplus . But the set V of all vectors $\vec{\alpha}$ with $0 \leq \alpha_k \leq 3$ form a vector space over the field with 2 elements $\{0, 1\}$. Here the addition of 2 vectors is given by \oplus and the multiplication by a scalar is given by

$$0 \cdot \vec{\alpha} = 0, \quad 1 \cdot \vec{\alpha} = \vec{\alpha}. \quad (20)$$

The dimension of the vector space is $2N$, and the condition (19) states that

$$W = \{\vec{\alpha} : \vec{\alpha} \in V, \sigma_{\vec{\alpha}} = 1\} \quad (21)$$

is a subspace of V . As such, W has a given dimension K , which means that W has 2^K elements, or in other words, that the 2^K rule holds.

By standard theorems of linear algebra, any subspace W can be extended to a maximal (non-trivial) subspace of dimension $2N - 1$ by adjoining appropriate additional basis elements. This can clearly be done in different ways. We therefore arrive to the set of maximal extensions of W . Clearly, the intersection of all the elements of this set reduces to W itself, leading to the claimed result that all PCE's can be obtained as intersections of maximal PCE's.

Finally, we may enumerate straightforwardly the subspaces W of dimension K . We do this in 2 steps: first, we evaluate $\mathcal{N}_{K,N}$, the number of all bases of K elements. Each of these corresponds to one subspace of dimension K , but each subspace corresponds to a number \mathcal{M}_K of different bases. The crucial point is that \mathcal{M}_K is independent of the subspace under consideration: \mathcal{M}_K simply

describes the number of linear maps of W onto itself. The total number $\mathcal{S}_{N,K}$ of subspaces of dimension K is therefore $\mathcal{N}_{N,K}/\mathcal{M}_K$.

To evaluate $\mathcal{N}_{N,K}$ we proceed by steps: the first element of the basis can be any non-zero element, of which the number is $2^{2N} - 1$. The second element must be chosen not belonging to the subspace generated by the first basis element. Of these there are $2^{2N} - 2$. Generally, for the basis element $m + 1$, we must choose from those which do not belong to the m dimensional space generated by the first m basis elements, so that one chooses from $2^{2N} - 2^m$. We thus have

$$\mathcal{N}_{N,K} = \prod_{m=0}^{K-1} (2^{2N} - 2^m). \quad (22)$$

On the other hand, the maps of a K -dimensional vector space W onto itself is described by a non-singular binary $K \times K$ matrix over the field $\{0,1\}$. To count these, we proceed as above: the first line is an arbitrary non-zero vector, of which there are $2^K - 1$. For the row $m + 1$ we must choose an arbitrary vector not belonging to those generated by the first m vectors, of which there are $2^K - 2^m$. This eventually yields

$$\mathcal{M}_K = \prod_{m=0}^{K-1} (2^K - 2^m). \quad (23)$$

From this follows that

$$\mathcal{S}_{N,K} = \prod_{m=0}^{K-1} \frac{2^{2N-m} - 1}{2^{K-m} - 1}. \quad (24)$$

An elementary test is $N = 3$ and $K = 2, 3$:

$$\mathcal{S}_{3,2} = \frac{(2^6 - 1)(2^5 - 1)}{(2^2 - 1)(2^1 - 1)} = \frac{63 \cdot 31}{3} = 651, \quad (25)$$

$$\mathcal{S}_{3,3} = \frac{(2^6 - 1)(2^5 - 1)(2^4 - 1)}{(2^3 - 1)(2^2 - 1)(2^1 - 1)} = \frac{63 \cdot 31 \cdot 15}{7 \cdot 3} = 1395, \quad (26)$$

which are indeed the values found numerically.

The symmetry suggested in the paper

$$\mathcal{S}_{N,K} = \mathcal{S}_{N,2N-K} \quad (27)$$

can also be proved with a bit of algebra from (24).